Types.dfy
@@ -1,15 +1,7 @@
 include "Auxiliary.dfy"
 
 module TypeMod{
-  /*type A(==)
-  type B(==)
-  type C(==)
-  type D(==)
-  type T(==)*/
-  const sizeT:nat := 1  // upper bound
-  const upperBound:nat    // hacer TypeMod abstract?
-  //function polynomial() : nat
-
+  const sizeT:nat := 1
 
   type Set<T(==)>{
 
@@ -17,81 +9,81 @@ module TypeMod{
   ghost function Size():nat
   {|Model()|*sizeT}
 
-  method Pick(ghost counter_in:nat) returns (e:T, ghost counter_out:nat)
+  method {:axiom} Pick(ghost counter_in:nat) returns (e:T, ghost counter_out:nat)
     requires Model() != {}
     ensures counter_out == counter_in + sizeT
     ensures e in Model()
   
-  method Empty(ghost counter_in:nat) returns (b:bool, ghost counter_out:nat)
+  method {:axiom} Empty(ghost counter_in:nat) returns (b:bool, ghost counter_out:nat)
     ensures b == (Model() == {})
     ensures counter_out == counter_in + 1
   
-  method Cardinality(ghost counter_in:nat) returns (size:int, ghost counter_out:nat)
+  method {:axiom} Cardinality(ghost counter_in:nat) returns (size:int, ghost counter_out:nat)
     ensures  size == |Model()|
     ensures counter_out == counter_in + 1
   
-  method Add(e:T, ghost counter_in:nat) returns (R:Set<T>, ghost counter_out:nat)
+  method {:axiom} Add(e:T, ghost counter_in:nat) returns (R:Set<T>, ghost counter_out:nat)
     ensures  R.Model() == Model() + {e}
     ensures if e in Model() then |R.Model()| == |Model()|
             else |R.Model()| == |Model()| + 1
     ensures counter_out == counter_in + sizeT
 
-  method Remove(e:T, ghost counter_in:nat) returns (R:Set<T>, ghost counter_out:nat)
+  method {:axiom} Remove(e:T, ghost counter_in:nat) returns (R:Set<T>, ghost counter_out:nat)
     ensures  R.Model() == Model() - {e}
     ensures if e !in Model() then |R.Model()| == |Model()|
             else |R.Model()| == |Model()| - 1
     ensures counter_out == counter_in + Size()
   
-  method Contains(e:T, ghost counter_in:nat) returns (b:bool, ghost counter_out:nat)
+  method {:axiom} Contains(e:T, ghost counter_in:nat) returns (b:bool, ghost counter_out:nat)
     ensures  b == (e in Model()) 
     ensures counter_out == counter_in + Size()
 
-  method Copy(ghost counter_in:nat) returns (R:Set<T>, ghost counter_out:nat)
+  method {:axiom} Copy(ghost counter_in:nat) returns (R:Set<T>, ghost counter_out:nat)
     ensures R.Model() == Model()
     ensures counter_out == counter_in + Size()
 
   }
 
 
-  type SetSet<T(==)>{
+  type SetSet<T(==)> {
    ghost function Model():set<set<T>>
-   ghost function maximumSizeElements():nat
+   ghost function {:axiom} maximumSizeElements():nat
    ensures forall s | s in Model() :: maximumSizeElements() >= |s|*sizeT
    ensures exists s :: s in Model() && maximumSizeElements() == |s|*sizeT
 
    ghost function Size():nat
     {|Model()|*maximumSizeElements()}
 
-  method Pick(ghost counter_in:nat) returns (e:Set<T>, ghost counter_out:nat)
+  method {:axiom} Pick(ghost counter_in:nat) returns (e:Set<T>, ghost counter_out:nat)
     requires Model() != {}
     ensures counter_out == counter_in + maximumSizeElements()
     ensures e.Model() in Model()
 
-  method Empty(ghost counter_in:nat) returns (b: bool, ghost counter_out:nat)
+  method {:axiom} Empty(ghost counter_in:nat) returns (b: bool, ghost counter_out:nat)
     ensures b == (Model() == {})
     ensures counter_out == counter_in + 1
   
-  method Cardinality(ghost counter_in:nat) returns (size: int, ghost counter_out:nat)
+  method {:axiom} Cardinality(ghost counter_in:nat) returns (size: int, ghost counter_out:nat)
     ensures  size == |Model()|
     ensures counter_out == counter_in + 1
   
-  method Add(e:Set<T>, ghost counter_in:nat) returns (R:SetSet<T>, ghost counter_out:nat)
+  method {:axiom} Add(e:Set<T>, ghost counter_in:nat) returns (R:SetSet<T>, ghost counter_out:nat)
     ensures  R.Model() == Model() + {e.Model()}
     ensures if e.Model() in Model() then |R.Model()| == |Model()|
             else |R.Model()| == |Model()| + 1
     ensures counter_out == counter_in + maximumSizeElements()
 
-  method Remove(e:Set<T>, ghost counter_in:nat) returns (R:SetSet<T>, ghost counter_out:nat)
+  method {:axiom} Remove(e:Set<T>, ghost counter_in:nat) returns (R:SetSet<T>, ghost counter_out:nat)
     ensures  R.Model() == Model() - {e.Model()}
     ensures if e.Model() !in Model() then |R.Model()| == |Model()|
             else |R.Model()| == |Model()| - 1
     ensures counter_out == counter_in + Size()
   
-  method Contains(e:Set<T>, ghost counter_in:nat) returns (b:bool, ghost counter_out:nat)
+  method {:axiom} Contains(e:Set<T>, ghost counter_in:nat) returns (b:bool, ghost counter_out:nat)
     ensures  b == (e.Model() in Model()) 
     ensures counter_out == counter_in + Size()
 
-  method Copy(ghost counter_in:nat) returns (R:SetSet<T>, ghost counter_out:nat)
+  method {:axiom} Copy(ghost counter_in:nat) returns (R:SetSet<T>, ghost counter_out:nat)
     ensures R.Model() == Model()
     ensures counter_out == counter_in + Size()
   }
@@ -100,11 +92,11 @@ module TypeMod{
   type SetSetSet<T(==)>{
    ghost function Model():set<set<set<T>>>
 
-   ghost function maximumSizeElements():nat
+   ghost function {:axiom} maximumSizeElements():nat
    ensures forall s | s in Model() :: maximumSizeElements() >= |s|*maximumSizeElements'()
    ensures exists s :: s in Model() && maximumSizeElements() == |s|*maximumSizeElements'()
 
-   ghost function maximumSizeElements'():nat
+   ghost function {:axiom} maximumSizeElements'():nat
    ensures forall s | s in Model() :: (forall s' | s' in s :: maximumSizeElements'() >= |s'|*sizeT)
    ensures exists s | s in Model() :: (exists s' | s' in s :: maximumSizeElements'() == |s'|*sizeT)
 
@@ -112,36 +104,36 @@ module TypeMod{
    ghost function Size():nat
     {|Model()|*maximumSizeElements()}
 
-  method Pick(ghost counter_in:nat) returns (e:SetSet<T>, ghost counter_out:nat)
+  method {:axiom} Pick(ghost counter_in:nat) returns (e:SetSet<T>, ghost counter_out:nat)
     requires Model() != {}
     ensures counter_out == counter_in + maximumSizeElements()
     ensures e.Model() in Model()
 
-  method Empty(ghost counter_in:nat) returns (b: bool, ghost counter_out:nat)
+  method {:axiom} Empty(ghost counter_in:nat) returns (b: bool, ghost counter_out:nat)
     ensures b == (Model() == {})
     ensures counter_out == counter_in + 1
   
-  method Cardinality(ghost counter_in:nat) returns (size: int, ghost counter_out:nat)
+  method {:axiom} Cardinality(ghost counter_in:nat) returns (size: int, ghost counter_out:nat)
     ensures  size == |Model()|
     ensures counter_out == counter_in + 1
   
-  method Add(e:SetSet<T>, ghost counter_in:nat) returns (R:SetSetSet<T>, ghost counter_out:nat)
+  method {:axiom} Add(e:SetSet<T>, ghost counter_in:nat) returns (R:SetSetSet<T>, ghost counter_out:nat)
     ensures  R.Model() == Model() + {e.Model()}
     ensures if e.Model() in Model() then |R.Model()| == |Model()|
             else |R.Model()| == |Model()| + 1
     ensures counter_out == counter_in + maximumSizeElements()
 
-  method Remove(e:SetSet<T>, ghost counter_in:nat) returns (R:SetSetSet<T>, ghost counter_out:nat)
+  method {:axiom} Remove(e:SetSet<T>, ghost counter_in:nat) returns (R:SetSetSet<T>, ghost counter_out:nat)
     ensures  R.Model() == Model() - {e.Model()}
     ensures if e.Model() !in Model() then |R.Model()| == |Model()|
             else |R.Model()| == |Model()| - 1
     ensures counter_out == counter_in + Size()
   
-  method Contains(e:SetSet<T>, ghost counter_in:nat) returns (b:bool, ghost counter_out:nat)
+  method {:axiom} Contains(e:SetSet<T>, ghost counter_in:nat) returns (b:bool, ghost counter_out:nat)
     ensures  b == (e.Model() in Model()) 
     ensures counter_out == counter_in + Size()
 
-  method Copy(ghost counter_in:nat) returns (R:SetSetSet<T>, ghost counter_out:nat)
+  method {:axiom} Copy(ghost counter_in:nat) returns (R:SetSetSet<T>, ghost counter_out:nat)
     ensures R.Model() == Model()
     ensures counter_out == counter_in + Size()
   }
@@ -153,40 +145,40 @@ module TypeMod{
   ghost function Size():nat
   {|Model()|*sizeT}
 
-  method Get(q:T0, ghost counter_in:nat) returns (a:T1, ghost counter_out:nat)
+  method {:axiom} Get(q:T0, ghost counter_in:nat) returns (a:T1, ghost counter_out:nat)
     requires Model() != map[]
     requires q in Model().Keys
     ensures counter_out == counter_in + sizeT
     ensures a == Model()[q]
 
-  method Add(q:T0, a:T1, ghost counter_in:nat) returns (R:Map<T0, T1>, ghost counter_out:nat)
+  method {:axiom} Add(q:T0, a:T1, ghost counter_in:nat) returns (R:Map<T0, T1>, ghost counter_out:nat)
     //requires !(q in Model().Keys)
     ensures counter_out == counter_in + sizeT
     ensures R.Model() == Model()[q := a]
 
-  method Remove(q:T0, ghost counter_in:nat) returns (R:Map<T0, T1>, ghost counter_out:nat)
+  method {:axiom} Remove(q:T0, ghost counter_in:nat) returns (R:Map<T0, T1>, ghost counter_out:nat)
     requires q in Model().Keys
     ensures counter_out == counter_in + sizeT
     ensures R.Model() == Model() - {q}
 
-  method Keys(ghost counter_in:nat) returns (keys:Set<T0>, ghost counter_out:nat)
+  method {:axiom} Keys(ghost counter_in:nat) returns (keys:Set<T0>, ghost counter_out:nat)
     ensures counter_out == counter_in + Size()
     ensures keys.Model() == Model().Keys
 
-  method Values(ghost counter_in:nat) returns (keys:Set<T1>, ghost counter_out:nat)
+  method {:axiom} Values(ghost counter_in:nat) returns (keys:Set<T1>, ghost counter_out:nat)
     ensures counter_out == counter_in + Size()
     ensures keys.Model() == Model().Values
 
-  method Items(ghost counter_in:nat) returns (keys:Set<(T0, T1)>, ghost counter_out:nat)
+  method {:axiom} Items(ghost counter_in:nat) returns (keys:Set<(T0, T1)>, ghost counter_out:nat)
     ensures counter_out == counter_in + Size()
     ensures keys.Model() == Model().Items
 
-  method HasKey(q:T0, ghost counter_in:nat) returns (b:bool, ghost counter_out:nat)
+  method {:axiom} HasKey(q:T0, ghost counter_in:nat) returns (b:bool, ghost counter_out:nat)
     ensures counter_out == counter_in + sizeT
     ensures b == (q in Model().Keys)
   
   /*
-  method Restrict(s:set<T0>, ghost counter_in:nat) returns (R:map<T0, T1>, ghost counter_out:nat)
+  method {:axiom} Restrict(s:set<T0>, ghost counter_in:nat) returns (R:map<T0, T1>, ghost counter_out:nat)
     requires s <= Model().Keys
     ensures counter_out == counter_in + Size()
     ensures R.Keys == s
@@ -203,39 +195,39 @@ module TypeMod{
   ghost function Size():nat
   {|Model()|*maximumSizeElements()}
 
-   ghost function maximumSizeElements():nat
+   ghost function {:axiom} maximumSizeElements():nat
    ensures forall s | s in Model().Keys :: maximumSizeElements() >= |s.Items|*sizeT
    ensures exists s :: s in Model() && maximumSizeElements() == |s.Items|*sizeT
 
-  method Get(q:Map<T0, T1>, ghost counter_in:nat) returns (a:T2, ghost counter_out:nat)
+  method {:axiom} Get(q:Map<T0, T1>, ghost counter_in:nat) returns (a:T2, ghost counter_out:nat)
     requires Model() != map[]
     requires q.Model() in Model().Keys
     ensures counter_out == counter_in + maximumSizeElements()
     ensures a == Model()[q.Model()]
 
-  method Add(q:Map<T0, T1>, a:T2, ghost counter_in:nat) returns (R:MapMap<T0, T1, T2>, ghost counter_out:nat)
+  method {:axiom} Add(q:Map<T0, T1>, a:T2, ghost counter_in:nat) returns (R:MapMap<T0, T1, T2>, ghost counter_out:nat)
     //requires !(q in Model().Keys)
     ensures counter_out == counter_in + maximumSizeElements()
     ensures R.Model() == Model()[q.Model() := a]
   
-  method Remove(q:Map<T0, T1>, ghost counter_in:nat) returns (R:MapMap<T0, T1, T2>, ghost counter_out:nat)
+  method {:axiom} Remove(q:Map<T0, T1>, ghost counter_in:nat) returns (R:MapMap<T0, T1, T2>, ghost counter_out:nat)
       requires q.Model() in Model().Keys
       ensures counter_out == counter_in + maximumSizeElements()
       ensures R.Model() == Model() - {q.Model()}
     
-  method Keys(ghost counter_in:nat) returns (keys:SetMap<T0, T1>, ghost counter_out:nat)
+  method {:axiom} Keys(ghost counter_in:nat) returns (keys:SetMap<T0, T1>, ghost counter_out:nat)
     ensures counter_out == counter_in + Size()
     ensures keys.Model() == Model().Keys
 
-  method Values(ghost counter_in:nat) returns (keys:Set<T2>, ghost counter_out:nat)
+  method {:axiom} Values(ghost counter_in:nat) returns (keys:Set<T2>, ghost counter_out:nat)
     ensures counter_out == counter_in + Size()
     ensures keys.Model() == Model().Values
 
-  method Items(ghost counter_in:nat) returns (keys:SetPairMap<T0, T1, T2>, ghost counter_out:nat)
+  method {:axiom} Items(ghost counter_in:nat) returns (keys:SetPairMap<T0, T1, T2>, ghost counter_out:nat)
     ensures counter_out == counter_in + Size()
     ensures keys.Model() == Model().Items
 
-  method HasKey(q:Map<T0, T1>, ghost counter_in:nat) returns (b:bool, ghost counter_out:nat)
+  method {:axiom} HasKey(q:Map<T0, T1>, ghost counter_in:nat) returns (b:bool, ghost counter_out:nat)
     ensures counter_out == counter_in + sizeT
     ensures b == (q.Model() in Model().Keys)
 
@@ -248,45 +240,45 @@ module TypeMod{
   ghost function Size():nat
   {|Model()|*maximumSizeElements()}
 
-  ghost function maximumSizeElements():nat
+  ghost function {:axiom} maximumSizeElements():nat
   ensures ((maximumSizeElements() >= maximumSizeKeys()) && (maximumSizeElements() == maximumSizeValues())) ||
           ((maximumSizeElements() == maximumSizeKeys()) && (maximumSizeElements() >= maximumSizeValues()))
 
-  ghost function maximumSizeKeys():nat
+  ghost function {:axiom} maximumSizeKeys():nat
   ensures forall s | s in Model().Keys :: maximumSizeKeys() >= |s.Items|*sizeT
   ensures exists s :: s in Model() && maximumSizeKeys() == |s.Items|*sizeT
 
-  ghost function maximumSizeValues():nat
+  ghost function {:axiom} maximumSizeValues():nat
   ensures forall setMap | setMap in Model().Values ::
           forall m | m in setMap :: maximumSizeValues() >= |m.Items|*sizeT
   ensures exists setMap | setMap in Model().Values ::
           exists m | m in setMap :: maximumSizeValues() == |m.Items|*sizeT
 
-  method Get(q:Map<T0, T1>, ghost counter_in:nat) returns (a:SetMap<T0, T1>, ghost counter_out:nat)
+  method {:axiom} Get(q:Map<T0, T1>, ghost counter_in:nat) returns (a:SetMap<T0, T1>, ghost counter_out:nat)
     requires Model() != map[]
     requires q.Model() in Model().Keys
     ensures counter_out == counter_in + maximumSizeElements()
     ensures a.Model() == Model()[q.Model()]
 
-  method Add(q:Map<T0, T1>, a:SetMap<T0, T1>, ghost counter_in:nat) returns (R:Map_Map_SetMap<T0, T1>, ghost counter_out:nat)
+  method {:axiom} Add(q:Map<T0, T1>, a:SetMap<T0, T1>, ghost counter_in:nat) returns (R:Map_Map_SetMap<T0, T1>, ghost counter_out:nat)
     //requires !(q in Model().Keys)
     ensures counter_out == counter_in + maximumSizeElements()
     ensures R.Model() == Model()[q.Model() := a.Model()]
   
-  method Remove(q:Map<T0, T1>, ghost counter_in:nat) returns (R:Map_Map_SetMap<T0, T1>, ghost counter_out:nat)
+  method {:axiom} Remove(q:Map<T0, T1>, ghost counter_in:nat) returns (R:Map_Map_SetMap<T0, T1>, ghost counter_out:nat)
       requires q.Model() in Model().Keys
       ensures counter_out == counter_in + maximumSizeElements()
       ensures R.Model() == Model() - {q.Model()}
     
-  method Keys(ghost counter_in:nat) returns (keys:SetMap<T0, T1>, ghost counter_out:nat)
+  method {:axiom} Keys(ghost counter_in:nat) returns (keys:SetMap<T0, T1>, ghost counter_out:nat)
     ensures counter_out == counter_in + Size()
     ensures keys.Model() == Model().Keys
 
-  method Values(ghost counter_in:nat) returns (keys:SetSetMap<T0, T1>, ghost counter_out:nat)
+  method {:axiom} Values(ghost counter_in:nat) returns (keys:SetSetMap<T0, T1>, ghost counter_out:nat)
     ensures counter_out == counter_in + Size()
     ensures keys.Model() == Model().Values
 
-  method HasKey(q:Map<T0, T1>, ghost counter_in:nat) returns (b:bool, ghost counter_out:nat)
+  method {:axiom} HasKey(q:Map<T0, T1>, ghost counter_in:nat) returns (b:bool, ghost counter_out:nat)
     ensures counter_out == counter_in + sizeT
     ensures b == (q.Model() in Model().Keys)
 
@@ -299,40 +291,40 @@ module TypeMod{
     ghost function Size():nat
     {|Model()|*maximumSizeElements()}
 
-    ghost function maximumSizeElements():nat
+    ghost function {:axiom} maximumSizeElements():nat
     ensures forall s | s in Model() :: maximumSizeElements() >= |s.Items|*sizeT
     ensures exists s :: s in Model() && maximumSizeElements() == |s.Items|*sizeT
 
-    method Pick(ghost counter_in:nat) returns (e:Map<T0, T1>, ghost counter_out:nat)
+    method {:axiom} Pick(ghost counter_in:nat) returns (e:Map<T0, T1>, ghost counter_out:nat)
       requires Model() != {}
       ensures counter_out == counter_in + maximumSizeElements()
       ensures e.Model() in Model()
     
-    method Empty(ghost counter_in:nat) returns (b:bool, ghost counter_out:nat)
+    method {:axiom} Empty(ghost counter_in:nat) returns (b:bool, ghost counter_out:nat)
       ensures b == (Model() == {})
       ensures counter_out == counter_in + 1
     
-    method Cardinality(ghost counter_in:nat) returns (size: int, ghost counter_out:nat)
+    method {:axiom} Cardinality(ghost counter_in:nat) returns (size: int, ghost counter_out:nat)
       ensures  size == |Model()|
       ensures counter_out == counter_in + 1
     
-    method Add(e:Map<T0, T1>, ghost counter_in:nat) returns (R:SetMap<T0, T1>, ghost counter_out:nat)
+    method {:axiom} Add(e:Map<T0, T1>, ghost counter_in:nat) returns (R:SetMap<T0, T1>, ghost counter_out:nat)
       ensures  R.Model() == Model() + {e.Model()}
       ensures if e.Model() in Model() then |R.Model()| == |Model()|
               else |R.Model()| == |Model()| + 1
       ensures counter_out == counter_in + Size()
 
-    method Remove(e:Map<T0, T1>, ghost counter_in:nat) returns (R:SetMap<T0, T1>, ghost counter_out:nat)
+    method {:axiom} Remove(e:Map<T0, T1>, ghost counter_in:nat) returns (R:SetMap<T0, T1>, ghost counter_out:nat)
       ensures  R.Model() == Model() - {e.Model()}
       ensures if e.Model() !in Model() then |R.Model()| == |Model()|
               else |R.Model()| == |Model()| - 1
       ensures counter_out == counter_in + Size()
     
-    method Contains(e:Map<T0, T1>, ghost counter_in:nat) returns (b:bool, ghost counter_out:nat)
+    method {:axiom} Contains(e:Map<T0, T1>, ghost counter_in:nat) returns (b:bool, ghost counter_out:nat)
       ensures  b == (e.Model() in Model()) 
       ensures counter_out == counter_in + Size()
 
-    method Copy(ghost counter_in:nat) returns (R:SetMap<T0, T1>, ghost counter_out:nat)
+    method {:axiom} Copy(ghost counter_in:nat) returns (R:SetMap<T0, T1>, ghost counter_out:nat)
       ensures R.Model() == Model()
       ensures counter_out == counter_in + Size()
 
@@ -349,36 +341,36 @@ type SetSetMap<T0(==), T1(==)>{
     // ensures forall s | s in Model() :: maximumSizeElements() >= |s.Items|*sizeT
     //ensures exists s :: s in Model() && maximumSizeElements() == |s.Items|*sizeT
 
-    method Pick(ghost counter_in:nat) returns (e:SetMap<T0, T1>, ghost counter_out:nat)
+    method {:axiom} Pick(ghost counter_in:nat) returns (e:SetMap<T0, T1>, ghost counter_out:nat)
       requires Model() != {}
       ensures counter_out == counter_in + maximumSizeElements()
       ensures e.Model() in Model()
     
-    method Empty(ghost counter_in:nat) returns (b:bool, ghost counter_out:nat)
+    method {:axiom} Empty(ghost counter_in:nat) returns (b:bool, ghost counter_out:nat)
       ensures b == (Model() == {})
       ensures counter_out == counter_in + 1
     
-    method Cardinality(ghost counter_in:nat) returns (size: int, ghost counter_out:nat)
+    method {:axiom} Cardinality(ghost counter_in:nat) returns (size: int, ghost counter_out:nat)
       ensures  size == |Model()|
       ensures counter_out == counter_in + 1
     
-    method Add(e:SetMap<T0, T1>, ghost counter_in:nat) returns (R:SetSetMap<T0, T1>, ghost counter_out:nat)
+    method {:axiom} Add(e:SetMap<T0, T1>, ghost counter_in:nat) returns (R:SetSetMap<T0, T1>, ghost counter_out:nat)
       ensures  R.Model() == Model() + {e.Model()}
       ensures if e.Model() in Model() then |R.Model()| == |Model()|
               else |R.Model()| == |Model()| + 1
       ensures counter_out == counter_in + Size()
 
-    method Remove(e:SetMap<T0, T1>, ghost counter_in:nat) returns (R:SetSetMap<T0, T1>, ghost counter_out:nat)
+    method {:axiom} Remove(e:SetMap<T0, T1>, ghost counter_in:nat) returns (R:SetSetMap<T0, T1>, ghost counter_out:nat)
       ensures  R.Model() == Model() - {e.Model()}
       ensures if e.Model() !in Model() then |R.Model()| == |Model()|
               else |R.Model()| == |Model()| - 1
       ensures counter_out == counter_in + Size()
     
-    method Contains(e:SetMap<T0, T1>, ghost counter_in:nat) returns (b:bool, ghost counter_out:nat)
+    method {:axiom} Contains(e:SetMap<T0, T1>, ghost counter_in:nat) returns (b:bool, ghost counter_out:nat)
       ensures  b == (e.Model() in Model()) 
       ensures counter_out == counter_in + Size()
 
-    method Copy(ghost counter_in:nat) returns (R:SetSetMap<T0, T1>, ghost counter_out:nat)
+    method {:axiom} Copy(ghost counter_in:nat) returns (R:SetSetMap<T0, T1>, ghost counter_out:nat)
       ensures R.Model() == Model()
       ensures counter_out == counter_in + Size()
 
@@ -391,72 +383,72 @@ type SetSetMap<T0(==), T1(==)>{
     ghost function Size():nat
     {|Model()|*maximumSizeElements()}
 
-    ghost function maximumSizeElements():nat
+    ghost function {:axiom} maximumSizeElements():nat
     ensures forall s | s in Model() :: maximumSizeElements() >= |s.0.Items|*sizeT
     ensures exists s :: s in Model() && maximumSizeElements() == |s.0.Items|*sizeT
 
-    method Pick(ghost counter_in:nat) returns (e:(Map<T0, T1>, T2), ghost counter_out:nat)
+    method {:axiom} Pick(ghost counter_in:nat) returns (e:(Map<T0, T1>, T2), ghost counter_out:nat)
       requires Model() != {}
       ensures counter_out == counter_in + maximumSizeElements()
       ensures exists m | m in Model() :: m.0 == e.0.Model() && m.1 == e.1
     
-    method Empty(ghost counter_in:nat) returns (b:bool, ghost counter_out:nat)
+    method {:axiom} Empty(ghost counter_in:nat) returns (b:bool, ghost counter_out:nat)
       ensures b == (Model() == {})
       ensures counter_out == counter_in + 1
     
-    method Cardinality(ghost counter_in:nat) returns (size: int, ghost counter_out:nat)
+    method {:axiom} Cardinality(ghost counter_in:nat) returns (size: int, ghost counter_out:nat)
       ensures  size == |Model()|
       ensures counter_out == counter_in + 1
     
-    method Add(e:(Map<T0, T1>, T2), ghost counter_in:nat) returns (R:SetPairMap<T0, T1, T2>, ghost counter_out:nat)
+    method {:axiom} Add(e:(Map<T0, T1>, T2), ghost counter_in:nat) returns (R:SetPairMap<T0, T1, T2>, ghost counter_out:nat)
       ensures  R.Model() == Model() + {(e.0.Model(), e.1)}
       ensures if (e.0.Model(), e.1) in Model() then |R.Model()| == |Model()|
               else |R.Model()| == |Model()| + 1
       ensures counter_out == counter_in + Size()
 
-    method Remove(e:(Map<T0, T1>, T2), ghost counter_in:nat) returns (R:SetPairMap<T0, T1, T2>, ghost counter_out:nat)
+    method {:axiom} Remove(e:(Map<T0, T1>, T2), ghost counter_in:nat) returns (R:SetPairMap<T0, T1, T2>, ghost counter_out:nat)
       ensures  R.Model() == Model() - {(e.0.Model(), e.1)}
       ensures if (e.0.Model(), e.1) !in Model() then |R.Model()| == |Model()|
               else |R.Model()| == |Model()| - 1
       ensures counter_out == counter_in + Size()
     
-    method Contains(e:(Map<T0, T1>, T2), ghost counter_in:nat) returns (b:bool, ghost counter_out:nat)
+    method {:axiom} Contains(e:(Map<T0, T1>, T2), ghost counter_in:nat) returns (b:bool, ghost counter_out:nat)
       ensures  b == ((e.0.Model(), e.1) in Model()) 
       ensures counter_out == counter_in + Size()
 
-    method Copy(ghost counter_in:nat) returns (R:SetPairMap<T0, T1, T2>, ghost counter_out:nat)
+    method {:axiom} Copy(ghost counter_in:nat) returns (R:SetPairMap<T0, T1, T2>, ghost counter_out:nat)
       ensures R.Model() == Model()
       ensures counter_out == counter_in + Size()
 
   }
 
 
- method NewSet(ghost counter_in:nat) returns (R:Set, ghost counter_out:nat)
+ method {:axiom} NewSet(ghost counter_in:nat) returns (R:Set, ghost counter_out:nat)
     ensures counter_out == counter_in +1
     ensures R.Model() == {}
   
-  method NewSetSet(ghost counter_in:nat) returns (R:SetSet, ghost counter_out:nat)
+  method {:axiom} NewSetSet(ghost counter_in:nat) returns (R:SetSet, ghost counter_out:nat)
     ensures counter_out == counter_in +1
     ensures R.Model() == {}
 
-  method NewSetSetSet(ghost counter_in:nat) returns (R:SetSetSet, ghost counter_out:nat)
+  method {:axiom} NewSetSetSet(ghost counter_in:nat) returns (R:SetSetSet, ghost counter_out:nat)
     ensures counter_out == counter_in +1
     ensures R.Model() == {}
 
-  method MakeSet<T(==)>(s:set<T>, ghost sizeT:nat, ghost counter_in:nat) returns (R:Set, ghost counter_out:nat)
+  method {:axiom} MakeSet<T(==)>(s:set<T>, ghost sizeT:nat, ghost counter_in:nat) returns (R:Set, ghost counter_out:nat)
     ensures counter_out == counter_in + sizeT*|s|
     ensures R.Model() == s
 
 
-  method NewMap(ghost counter_in:nat) returns (R:Map, ghost counter_out:nat)
+  method {:axiom} NewMap(ghost counter_in:nat) returns (R:Map, ghost counter_out:nat)
     ensures counter_out == counter_in +1
     ensures R.Model() == map[]
 
-  method NewMapMap(ghost counter_in:nat) returns (R:MapMap, ghost counter_out:nat)
+  method {:axiom} NewMapMap(ghost counter_in:nat) returns (R:MapMap, ghost counter_out:nat)
     ensures counter_out == counter_in +1
     ensures R.Model() == map[]
 
-  method MakeMap<A(==), B(==)>(s:map<A, B>, ghost sizeT:nat, ghost counter_in:nat) returns (R:Map<A, B>, ghost counter_out:nat)
+  method {:axiom} MakeMap<A(==), B(==)>(s:map<A, B>, ghost sizeT:nat, ghost counter_in:nat) returns (R:Map<A, B>, ghost counter_out:nat)
     ensures counter_out == counter_in + sizeT*|s|
     ensures R.Model() == s
 
